[DOC]

transformations/Class2Relational/utils/TraceUtils.v
@@ -5,6 +5,8 @@ Require Import Coq.Arith.Gt.
 Require Import Coq.Arith.EqNat.
 Require Import List.
 
+Open Scope string_scope.
+
 Require Import core.utils.Utils.
 Require Import core.Semantics.
 Require Import core.Certification.
@@ -17,38 +19,46 @@ Require Import transformations.Class2Relational.RelationalMetamodel.
 
 From transformations.Class2Relational Require Tactics.
 
+Import TraceLink.
 
-(** Utilities on traces *)
+(** * Utilities on traces built by the Class2Relational transformation. *)
 
-Inductive CoherentTrace : TraceLink.TraceLink -> Prop :=
+
+Inductive CoherentTraceLink : TraceLink -> Prop :=
 
  | ct_class :
-   forall t,
-     CoherentTrace 
-       (TraceLink.buildTraceLink 
-          ([ClassElement t], 0, "tab"%string)
+   forall (c:Class_t),
+     CoherentTraceLink 
+       (buildTraceLink 
+          ([ClassElement c], 0, "tab")
           (TableElement
              {|
-               table_id := class_id t; 
-               table_name := class_name t
+               table_id := c.(class_id); 
+               table_name := c.(class_name) 
              |}))
 
  | ct_attribute :
-   forall a,
-     CoherentTrace
-       (TraceLink.buildTraceLink 
-          ([AttributeElement a], 0, "col"%string)
+   forall (a:Attribute_t),
+     CoherentTraceLink
+       (buildTraceLink 
+          ([AttributeElement a], 0, "col")
           (ColumnElement
              {|
-               column_id := attr_id a ;
-               column_name :=  attr_name a 
+               column_id := a.(attr_id) ;
+               column_name :=  a.(attr_name) 
              |})).
 
+
+Definition wf t : Prop := 
+  List.Forall CoherentTraceLink t.
+
+(** Traces built by the Class2Relational transformation are well-formed. *)
 Lemma trace_wf cm :
-  Forall CoherentTrace (trace Class2Relational cm).
+  wf (trace Class2Relational cm).
 Proof.
   unfold trace.
   unfold allTuples.
+  unfold wf.
   apply Forall_flat_map.
   simpl.
   unfold prod_cons.
@@ -59,57 +69,59 @@ Proof.
   apply Forall_forall.
   intro r.
   intro H2.
+
+  (* remove [nil] in H (l cannot be nil)*)
   apply in_app_or in H.
   destruct_or H.
-  2:{ simpl in *.
-      remove_or_false H.
-      subst l.
-      simpl in *.
-      contradiction.
+  2:{ 
+    apply ListUtils.in_singleton in H ; subst l. 
+    simpl in *. contradiction.
   }
+  (* done *)
+
   apply in_flat_map in H.
   destruct H as (e & H3 & H4).
-  simpl in *.
-  remove_or_false H4.
-  subst l.
-  simpl in *.
+  simpl map in H4.
+  apply ListUtils.in_singleton in H4 ; subst l.
+
   unfold matchPattern in H2.
   apply filter_In in H2.
   destruct H2 as [H4 H5].
 
   
   Tactics.destruct_In_two ; simpl in * ; Tactics.deduce_element_kind_from_guard.
-  { repeat constructor. }  
-  { repeat constructor. }  
+  { (* rule 1 *) compute. constructor. constructor. constructor. }  
+  { (* rule 2 *) compute. constructor. constructor. constructor. }  
 Qed.
 
 
+Notation match_source s  :=
+  (fun (t:TraceLink) => 
+     match s with (e,i,n) =>
+                    ((Semantics.list_beq _
+                        TransformationConfiguration.SourceElement_eqb
+                        (TraceLink_getSourcePattern t)
+                        e) 
+                     && beq_nat (TraceLink_getIterator t) i
+                     && String.eqb (TraceLink_getName t) n)%bool
+     end).
 
-Lemma in_find_5bis l : 
-  Forall CoherentTrace l ->
-  forall t,
-    In (TraceLink.buildTraceLink
-          ([ClassElement t], 0, "tab"%string)
-          (TableElement {| table_id := class_id t; table_name := class_name t |})) l ->
+Lemma in_find_5bis t : 
+  wf t ->
+  forall c,
+    In (buildTraceLink
+          ([ClassElement c], 0, "tab")
+          (TableElement {| table_id := c.(class_id); table_name := c.(class_name)  |})) t ->
     exists r1 , 
-      find
-        (fun tl : TraceLink.TraceLink =>
-           (Semantics.list_beq
-              (Metamodel.ElementType
-                 TransformationConfiguration.SourceMetamodel)
-              TransformationConfiguration.SourceElement_eqb
-              (TraceLink.TraceLink_getSourcePattern tl)
-              (singleton (ClassElement t)) &&
-              (TraceLink.TraceLink_getIterator tl =? 0) &&
-              (TraceLink.TraceLink_getName tl =? "tab")%string)%bool) l = 
-        Some (TraceLink.buildTraceLink r1 (TableElement {| table_id := class_id t; table_name := class_name t |})).
+      find (match_source ([ClassElement c], 0, "tab")) t = 
+        Some (buildTraceLink r1 (TableElement {| table_id := c.(class_id); table_name := c.(class_name) |})).
 Proof.
-  induction l ; intros C t IN1 ; [ simpl in IN1 ; contradict IN1 | ].
+  induction t ; intros C c IN1 ; [ simpl in IN1 ; contradict IN1 | ].
   simpl.
   apply in_inv in IN1. 
-  compare a (TraceLink.buildTraceLink ([ClassElement t], 0, "tab"%string)
+  compare a (buildTraceLink ([ClassElement c], 0, "tab")
           (TableElement
-             {| table_id := class_id t; table_name := class_name t |})). 
+             {| table_id := c.(class_id); table_name := c.(class_name) |})). 
 
 
   { (* case where the class/table is the first element of the list : no induction *)
@@ -131,13 +143,13 @@ Proof.
     { (* class/table *)
       destruct_or IN1 ; [ contradict D ; assumption | ].
 
-      destruct (IHl H0 t) ; [  exact IN1 | ].
+      destruct (IHt H0 c) ; [  exact IN1 | ].
       unfold TransformationConfiguration.SourceElement_eqb .
       unfold Metamodel.elements_eqdec.
       unfold TransformationConfiguration.SourceMetamodel.
       unfold C2RConfiguration. simpl.
       repeat rewrite Bool.andb_true_r.
-      destruct (beq_Class t0 t) eqn:BEQ.
+      destruct (beq_Class c0 c) eqn:BEQ.
       {  apply lem_beq_Class_id in BEQ ; subst ; eauto.  }
       {
         simpl in H.
@@ -154,7 +166,7 @@ Proof.
     { (* attribute/column*)
       destruct_or IN1.
       { contradict IN1. exact D. }
-      destruct (IHl H0 t) ; [  exact IN1 | ].
+      destruct (IHt H0 c) ; [  exact IN1 | ].
       unfold TransformationConfiguration.SourceElement_eqb .
       unfold Metamodel.elements_eqdec.
       unfold TransformationConfiguration.SourceMetamodel.
@@ -170,37 +182,46 @@ Qed.
         
 
       
-Lemma in_resolve_4bis  l t cm : 
-  Forall CoherentTrace l ->
-  In (TraceLink.buildTraceLink
-        ([ClassElement t], 0, "tab"%string)
+Lemma in_resolve_4bis t c cm : 
+  wf t ->
+  In (buildTraceLink
+        ([ClassElement c], 0, "tab")
         (TableElement
-           {| table_id := class_id t; table_name := class_name t |})) l ->
-  resolveIter l cm "tab"
-    (singleton (ClassElement t)) 0 = Some (TableElement {| table_id := class_id t; table_name := class_name t |}).
+           {| table_id := c.(class_id); table_name := c.(class_name) |})) t ->
+  resolveIter t cm "tab" (singleton (ClassElement c)) 0 = 
+    Some (TableElement {| table_id := c.(class_id); table_name := c.(class_name) |}).
 Proof.
   unfold resolveIter. 
+  (* FIXME : in resolveIter, introduce match_source *)
   intros C IN1.
-  specialize (in_find_5bis l C t IN1) ; intro T5 ; clear IN1.
-  
+  specialize (in_find_5bis t C c IN1) ; intro T5 ; clear IN1.
   destruct T5 as (t1 & IN1).
+  unfold singleton.
   rewrite IN1.
-  unfold TraceLink.TraceLink_getTargetElement.
+  unfold TraceLink_getTargetElement.
   destruct t1.
   destruct p.
   reflexivity.
 Qed.
 
-Lemma in_trace_3  e (cm : ClassModel) : 
-  In (ClassElement e) cm.(modelElements) -> 
+Lemma in_trace_3 c (cm : ClassModel) : 
+  In (ClassElement c) cm.(modelElements) -> 
   In 
-    (TraceLink.buildTraceLink ([ClassElement e],0,"tab"%string) (TableElement {| table_id := class_id e; table_name := class_name e |})) 
+    (buildTraceLink 
+       ([ClassElement c],0,"tab") 
+       (TableElement 
+          {| 
+            table_id := c.(class_id); 
+            table_name := c.(class_name) 
+          |}
+         )
+    ) 
     (trace Class2Relational cm).
 Proof.
   intro IN1.
   unfold trace.
   apply in_flat_map.
-  exists ([ClassElement e]).
+  exists ([ClassElement c]).
   split.
   { apply Tactics.allModelElements_allTuples ; auto. } 
   { compute. left. reflexivity. }
